ProofLibrary/AlternativeMatches.lean
@@ -1,0 +1,127 @@
+import ProofLibrary.SubstitutionAndHomomorphismBasics
+import ProofLibrary.Trigger
+
+variable {sig : Signature} [DecidableEq sig.P] [DecidableEq sig.C] [DecidableEq sig.V]
+
+namespace GroundTermMapping
+
+  def isAlternativeMatch (h_alt : GroundTermMapping sig) (trg : PreTrigger sig) (disj_index : Fin trg.result.length) (fs : FactSet sig) : Prop :=
+    (h_alt.isHomomorphism (trg.result.get disj_index) fs) ∧
+    (∀ t, t ∈ trg.rule.frontier.map trg.subs -> h_alt t = t) ∧
+    (∃ n, (n ∈ (trg.result.get disj_index).terms) ∧ (¬ n ∈ (h_alt.applyFactSet (trg.result.get disj_index)).terms))
+
+end GroundTermMapping
+
+namespace PreTrigger
+
+  -- TODO: cleanup the proof; seems like we need lemmas on PreTrigger and Substitution Interaction (likely also useful elsewhere)
+  theorem satisfied_of_alternativeMatch (trg : PreTrigger sig) (fs : FactSet sig) : ∀ (h_alt : GroundTermMapping sig) (disj_index : Fin trg.result.length), h_alt.isAlternativeMatch trg disj_index fs -> trg.satisfied fs := by
+    intro h_alt disj_index is_alt_match
+    exists ⟨disj_index.val, by have isLt := disj_index.isLt; rw [PreTrigger.head_length_eq_mapped_head_length]; unfold PreTrigger.result at isLt; simp at isLt; exact isLt⟩
+    exists (h_alt ∘ trg.apply_to_var_or_const disj_index ∘ VarOrConst.var)
+    constructor
+    . intro v v_in_frontier
+      simp only [Function.comp_apply]
+      simp [PreTrigger.apply_to_var_or_const, PreTrigger.apply_to_skolemized_term, PreTrigger.skolemize_var_or_const, VarOrConst.skolemize, v_in_frontier]
+      apply is_alt_match.right.left
+      simp
+      exists v
+    . intro f f_mem
+      apply is_alt_match.left.right
+      rw [← List.inIffInToSet] at f_mem
+      unfold GroundSubstitution.apply_function_free_conj at f_mem
+      simp at f_mem
+      simp [PreTrigger.result, PreTrigger.mapped_head]
+      unfold GroundTermMapping.applyFactSet
+      rcases f_mem with ⟨a, a_mem, a_eq⟩
+      exists trg.apply_to_function_free_atom disj_index a
+      constructor
+      . rw [← List.inIffInToSet]
+        simp
+        exists a
+      . unfold PreTrigger.apply_to_function_free_atom
+        unfold GroundTermMapping.applyFact
+        simp
+        unfold GroundSubstitution.apply_function_free_atom at a_eq
+        rw [← a_eq]
+        simp [PreTrigger.apply_to_var_or_const]
+        intro t t_mem
+        unfold PreTrigger.apply_to_skolemized_term
+        unfold PreTrigger.skolemize_var_or_const
+        simp [GroundSubstitution.apply_var_or_const]
+        cases t with
+        | const c => simp [VarOrConst.skolemize, GroundSubstitution.apply_skolem_term]; apply is_alt_match.left.left (GroundTerm.const c)
+        | var v => simp
+
+  theorem alternativeMatch_of_satisfied (trg : PreTrigger sig) (fs : FactSet sig) (disj_index : Fin trg.result.length) (gt : GroundTerm sig) (gt_in_res_but_not_fs : gt ∈ (trg.result.get disj_index).terms ∧ ¬ gt ∈ fs.terms) : trg.satisfied_for_disj fs ⟨disj_index, by rw [PreTrigger.head_length_eq_mapped_head_length]; have isLt := disj_index.isLt; unfold PreTrigger.result at isLt; simp at isLt; exact isLt⟩ -> ∃ (h_alt : GroundTermMapping sig), h_alt.isAlternativeMatch trg disj_index fs := by
+    intro satisfied
+    rcases satisfied with ⟨s, s_frontier, s_subs⟩
+
+    let h_alt : GroundTermMapping sig := fun t =>
+      if t ∈ trg.rule.frontier.map trg.subs then t else match t with
+        | .leaf c => t
+        | .inner skolem_fs _ => s skolem_fs.var
+
+    have : h_alt.applyFactSet (trg.result.get disj_index) ⊆ fs := by
+      intro f f_mem
+      apply s_subs
+      unfold GroundTermMapping.applyFactSet at f_mem
+      rcases f_mem with ⟨f', f'_mem, f'_eq⟩
+      simp [PreTrigger.result, PreTrigger.mapped_head] at f'_mem
+      rw [← List.inIffInToSet] at f'_mem
+      simp at f'_mem
+      rcases f'_mem with ⟨a, a_mem, a_eq⟩
+
+      rw [← List.inIffInToSet]
+      simp [GroundSubstitution.apply_function_free_conj]
+      exists a
+      constructor
+      . exact a_mem
+      . rw [← f'_eq, ← a_eq]
+        simp [GroundSubstitution.apply_function_free_atom, GroundTermMapping.applyFact, PreTrigger.apply_to_function_free_atom]
+        intro voc voc_mem
+        cases voc with
+        | const c =>
+          simp [GroundSubstitution.apply_var_or_const, PreTrigger.apply_to_var_or_const, PreTrigger.skolemize_var_or_const, VarOrConst.skolemize, PreTrigger.apply_to_skolemized_term, GroundSubstitution.apply_skolem_term]
+          simp [h_alt]
+        | var v =>
+          simp [GroundSubstitution.apply_var_or_const]
+          cases Decidable.em (v ∈ trg.rule.frontier) with
+          | inl v_in_frontier =>
+            simp [PreTrigger.apply_to_var_or_const, PreTrigger.skolemize_var_or_const, VarOrConst.skolemize, PreTrigger.apply_to_skolemized_term, GroundSubstitution.apply_skolem_term]
+            simp [v_in_frontier, h_alt]
+            have : ∃ a, a ∈ trg.rule.frontier ∧ trg.subs a = trg.subs v := by exists v
+            simp [this]
+            apply s_frontier
+            exact v_in_frontier
+          | inr v_not_in_frontier =>
+            simp only [h_alt]
+            have : ¬ trg.apply_to_var_or_const disj_index.val (VarOrConst.var v) ∈ trg.rule.frontier.map trg.subs := by
+              apply PreTrigger.result_term_not_in_frontier_image_of_var_not_in_frontier
+              exact v_not_in_frontier
+            simp [this]
+            simp [PreTrigger.apply_to_var_or_const, PreTrigger.skolemize_var_or_const, VarOrConst.skolemize, PreTrigger.apply_to_skolemized_term, GroundSubstitution.apply_skolem_term]
+            simp [v_not_in_frontier]
+
+    exists h_alt
+    constructor
+    . constructor
+      . intro t; cases t with
+        | leaf c => simp [h_alt]
+        | inner _ _ => simp
+      . exact this
+    constructor
+    . intro t ht; simp only [h_alt, ht]; simp
+    . exists gt
+      constructor
+      . exact gt_in_res_but_not_fs.left
+      . intro contra
+        apply gt_in_res_but_not_fs.right
+        rcases contra with ⟨f, f_mem, gt_mem⟩
+        exists f
+        constructor
+        . apply this; exact f_mem
+        . exact gt_mem
+
+end PreTrigger
+
